```latex
\documentclass{article}
\usepackage{amsmath}
\usepackage{amssymb}
\usepackage{graphicx}

\begin{document}

% Page 1
\section*{Homework 2}

\subsection*{1)}
\begin{align*}
P(A) &= 0.3 \\
P(B) &= 0.4 \\
P(A \cap B) &= 0.2 \\
\text{a) } P(A \cup B) &= P(A) + P(B) - P(A \cap B) \\
&= 0.3 + 0.4 - 0.2 = 0.5 \\
\text{b) If } A \text{ and } B \text{ are independent, } & \\
P(A) \cdot P(B) &= P(A \cap B) \\
0.3 \cdot 0.4 &= 0.2 \quad \checkmark \\
\text{c) } P(A^c \cap B) &= P(B) - P(A \cap B) \\
&= 0.4 - 0.2 = 0.2
\end{align*}

\subsection*{2)}
\begin{align*}
f_X(x) &=
\begin{cases} 
2x & 0 \leq x \leq 1 \\
0 & \text{otherwise} 
\end{cases} \\
\text{a) } \ell(x) &= \int_{-\infty}^{\infty} x f(x) \, dx \\
&= \int_0^1 2x^2 \, dx \\
&= \left. \frac{2}{3} x^3 \right|_0^1 \\
&= \frac{2}{3} \\
\text{Var}(X) &= \mathbb{E}(X^2) - \ell(x)^2 \\
\mathbb{E}(X^2) &= \int_{-\infty}^{\infty} x^2 f(x) \, dx \\
&= \int_0^1 2x^3 \, dx \\
&= \left. \frac{1}{2} x^4 \right|_0^1 \\
&= \frac{1}{2} \\
\text{Var}(X) &= \frac{1}{2} - \left( \frac{2}{3} \right)^2 \\
&= \frac{1}{2} - \frac{4}{9} \\
&= \frac{1}{18}
\end{align*}

\subsection*{b)}
\begin{align*}
\mathbb{P}(X = x) &= \phi^x (1 - \phi)^{1-x} \\
\mathbb{P}(X = 1) &= \phi \\
\mathbb{P}(X = 0) &= 1 - \phi \\
\mathcal{L}(x) &= \frac{1}{2} x \cdot \mathbb{P}(X = x) \\
&= 0 \cdot (1 - \phi) + 1 \cdot \phi \\
&= \phi \\
\text{Var}(X) &= \mathbb{E}(x^2) - \mathcal{L}(x)^2 \\
\mathbb{E}(x^2) &= \frac{1}{2} x^2 \cdot \mathbb{P}(X = x) \\
&= 0 \cdot (1 - \phi) + 1 \cdot \phi \\
&= \phi \\
\text{Var}(X) &= \phi - \phi^2 \\
&= \phi (1 - \phi)
\end{align*}

% Page 2
\subsection*{3)}
\begin{align*}
f_{xy}(x, y) &=
\begin{cases} 
6xy & 0 \leq x \leq 1, \; 0 \leq y \leq 1 
\end{cases} \\
\text{a) } f_x(x) &= \int_0^1 6xy \, dy \\
&= 6x \left[ \frac{y^2}{2} \right]_0^1 \\
&= 3x \\
\text{Similarly, } f_y(y) &= 3y \\
\text{b) } f_x(x) \cdot f_y(y) &= 9xy \neq 6xy \\
&\text{Not independent}
\end{align*}

\subsection*{4)}
\begin{align*}
\text{Event } A: \quad P(5 \text{ or } 6) &= \frac{2}{6} \\
\text{Event } B: \quad P((3,6), (4,6), (5,6), (6,6), (6,5), (6,4), (6,3), (5,4), (5,5), (4,5)) &= \frac{10}{36} \\
P(B|A) &= \frac{P(A \cap B)}{P(A)} \\
|A \cap B| &= \{(5,4), (5,5), (5,6), (6,3), (6,4), (6,5), (6,6)\} \\
&= 7 \\
\frac{\frac{7}{36}}{\frac{2}{6}} &= \frac{7}{12}
\end{align*}

% Page 3
\subsection*{5)}
\begin{align*}
\text{r.v. } X \text{ with } Y &= (1-x)^{1/3} \\
\text{pdf } f(x) &= 3(1-x)^2 \\
Y^{1/3} &= 1-x \\
X &= 1-Y^{1/3} \\
\frac{dX}{dY} &= -\frac{1}{3} Y^{-2/3} \\
f_Y(y) &= f_X(1-Y^{1/3}) \left| \frac{dy}{dx} \right| \\
&= 3(1-(1-Y^{1/3}))^2 \cdot \frac{1}{3} Y^{-2/3} \left| \frac{dy}{dx} \right| \\
&= 3(Y^{1/3})^2 \cdot \frac{1}{3} Y^{-2/3} \\
&= 1 \\
f_Y(y) &=
\begin{cases} 
1 & 0 \leq y \leq 1 \\
0 & \text{otherwise} 
\end{cases}
\end{align*}

\subsection*{6)}
\begin{align*}
\text{Cov} \left( \sum_{i=1}^{n} a_i X_i, \sum_{j=1}^{n} a_j X_j \right) &= \sum_{i=1}^{n} \sum_{j=1}^{n} a_i a_j \text{Cov}(X_i, X_j) = a^T S a \\
Y &= \sum_{i=1}^{n} a_i X_i \quad Z = \sum_{j=1}^{n} a_j X_j \\
t(\mathbf{Y}) &= \mathbb{E} \left( \sum_{i=1}^{n} a_i X_i \right) = \sum_{i=1}^{n} a_i t(X_i) \\
t(\mathbf{Z}) &= \sum_{j=1}^{n} a_j t(X_j) \\
t(\mathbf{Y Z}) &= \mathbb{E} \left( \left( \sum_{i=1}^{n} a_i X_i \right) \left( \sum_{j=1}^{n} a_j X_j \right) \right)
\end{align*}

% Page 4
\begin{align*}
&= \mathbb{E} \left( \left( \sum_{i=1}^{n} \sum_{j=1}^{n} a_i a_j X_i X_j \right) \right) \\
&= \sum_{i=1}^{n} a_i a_i \mathbb{E}(X_i X_j) \\
\text{Cov}(Y, Z) &= \mathbb{E}(YZ) - \mathbb{E}(Y) \mathbb{E}(Z) \\
&= \sum_{i=1}^{n} \sum_{j=1}^{n} a_i a_j \mathbb{E}(X_i X_j) - \sum_{i=1}^{n} a_i \mathbb{E}(X_i) \sum_{j=1}^{n} a_j \mathbb{E}(X_j) \\
&= \sum_{i=1}^{n} \sum_{j=1}^{n} a_i a_j \mathbb{E}(X_i X_j) - \sum_{i=1}^{n} \sum_{j=1}^{n} a_i a_j \mathbb{E}(X_i) \mathbb{E}(X_j) \\
&= \sum_{i=1}^{n} \sum_{j=1}^{n} a_i a_j \left( \mathbb{E}(X_i X_j) - \mathbb{E}(X_i) \mathbb{E}(X_j) \right) \\
&= \sum_{i=1}^{n} \sum_{j=1}^{n} a_i a_j \text{Cov}(X_i, X_j) \\
a^T S a &= \sum_{i=1}^{n} \sum_{j=1}^{n} a_i S_{ij} a_j = \sum_{i=1}^{n} \sum_{j=1}^{n} a_i a_j \text{Cov}(X_i, X_j)
\end{align*}

% Page 5
\subsection*{1)}
\begin{align*}
f(x) &= \log(1 + e^x) \\
\sigma(x) &= \frac{e^x}{1 + e^x} \\
\text{① } \frac{d}{dx} f(x) &= \frac{1}{1 + e^x} \cdot \frac{d}{dx}(1 + e^x) = \frac{e^x}{1 + e^x} \\
\text{② } \frac{d \sigma(x)}{dx} &= \frac{\frac{d}{dx} e^x \cdot (1 + e^x) - e^x \cdot \frac{d}{dx}(1 + e^x)}{(1 + e^x)^2} \\
&= \frac{e^x (1 + e^x) - e^x e^x}{(e^x + 1)^2} \\
&= \frac{e^x}{(1 + e^x)^2} \\
&= \sigma(x) \cdot \frac{1}{1 + e^x} \\
&= \sigma(x) \cdot \frac{1 + e^x}{1 + e^x} - \frac{e^x}{1 + e^x} \\
&= \sigma(x) (1 - \sigma(x))
\end{align*}

% Page 6
\subsection*{3)}
\begin{align*}
\log(\sigma(x)) &= -f(x) \\
\log\left(\frac{1}{1+e^x}\right) &= \log\left(e^{-x}\right) - \log(1+e^x) \\
&= -x - \log(1+e^x) \\
&= x - f(x) \\
&= -f(x)
\end{align*}

\subsection*{4)}
\begin{align*}
1 - \sigma(x) &= 1 - \frac{e^x}{e^x+1} = \frac{e^x+1 - e^x}{e^x+1} = \frac{1}{e^x+1} \\
\sigma(-x) &= \frac{e^{-x}}{1+e^{-x}} = \frac{1}{1+e^x} \\
\sigma(-x) &= 1 - \sigma(x)
\end{align*}

\subsection*{5)}
\begin{align*}
\sigma^{-1}(x) &= \log\left(\frac{x}{1-x}\right) \\
e^y &= \frac{x}{1-x} \\
x &= e^y(1-x) \\
e^y(1-x) &= x \\
e^y &= \frac{x}{1-x} \\
y &= \log\left(\frac{x}{1-x}\right)
\end{align*}

% Page 7
\subsection*{6)}
\begin{align*}
\forall x \geq 0 \quad f^{-1}(x) &= \ln\left(C \exp(x) - 1\right) \\
y &= \ln(1 + e^x) \\
C^x &= 1 + e^x \\
e^x &= e^{x - 1} \\
x &= \ln(C^x - 1) \\
f^{-1}(x) &= \ln(C^x - 1)
\end{align*}

\subsection*{7)}
\begin{align*}
f(x) &= \int_{-\infty}^{x} C \ln(y) \, dy \\
&= \int_{-\infty}^{x} \frac{C}{1 + e^y} \, dy \\
u &= 1 + e^y \\
du &= e^y \, dy \\
\int \frac{1}{u} \, du &= \ln(1 + e^x) \bigg|_{-\infty}^{x} \\
&= \ln(1 + e^x) - \ln(1 + e^{-\infty}) \\
&= \ln(1 + e^x) - \ln(1) \\
&= \ln(1 + e^x)
\end{align*}

% Page 8
\subsection*{8)}
\begin{align*}
f(x) - f(-x) &= x \\
f(x) - f(-x) &= \ln(1 + e^x) - \ln(1 + e^{-x}) \\
&= \ln\left(\frac{1 + e^x}{1 + e^{-x}}\right) = \ln\left(\frac{C^x + 1}{C^x}\right) \\
&= \log(1 + e^x) - \left( \log(e^x + 1) - x \right) \\
&= x
\end{align*}

\end{document}
```