% LaTeX output generated from Hw2.pdf
% Generated on: 2025-06-28 16:06:59
% Using Anthropic Claude Sonnet 4

```latex
\documentclass{article}
\usepackage{amsmath}
\usepackage{amssymb}
\usepackage{geometry}
\geometry{margin=1in}

\begin{document}

\section*{Homework 2}

\subsection*{Problem 1}
Given: $P(A) = 0.3$, $P(B) = 0.4$, $P(A \cap B) = 0.2$

\textbf{a)} $P(A \cup B) = P(A) + P(B) - P(A \cap B) = 0.3 + 0.4 - 0.2 = 0.5$

\textbf{b)} If $A$ and $B$ are independent, then $P(A) \cdot P(B) = P(A \cap B)$
$0.3 \cdot 0.4 = 0.12 \neq 0.2$
Therefore, $A$ and $B$ are not independent.

\textbf{c)} $P(A^c \cap B) = P(B) - P(A \cap B) = 0.4 - 0.2 = 0.2$

\subsection*{Problem 2}
$f_X(x) = \begin{cases} 2x & 0 \leq x \leq 1 \\ 0 & \text{otherwise} \end{cases}$

\textbf{a)} $E(X) = \int_{-\infty}^{\infty} x f(x) dx = \int_0^1 x \cdot 2x dx = \int_0^1 2x^2 dx = \frac{2x^3}{3}\Big|_0^1 = \frac{2}{3}$

$\text{Var}(X) = E(X^2) - [E(X)]^2$

$E(X^2) = \int_{-\infty}^{\infty} x^2 f(x) dx = \int_0^1 x^2 \cdot 2x dx = \int_0^1 2x^3 dx = \frac{2x^4}{4}\Big|_0^1 = \frac{1}{2}$

$\text{Var}(X) = \frac{1}{2} - \left(\frac{2}{3}\right)^2 = \frac{1}{2} - \frac{4}{9} = \frac{9-8}{18} = \frac{1}{18}$

\textbf{b)} $P(X = x) = p^x(1-p)^{1-x}$ for $x \in \{0,1\}$

$P(X = 1) = p^1(1-p)^0 = p$

$P(X = 0) = p^0(1-p)^1 = (1-p)$

$E(X) = \sum x P(X = x) = 0(1-p) + 1(p) = p$

$E(X^2) = \sum x^2 P(X = x) = 0^2(1-p) + 1^2(p) = p$

$\text{Var}(X) = E(X^2) - [E(X)]^2 = p - p^2 = p(1-p)$

\subsection*{Problem 3}
$f_{X,Y}(x,y) = 6xy$ for $0 \leq x \leq 1, 0 \leq y \leq 1$

\textbf{a)} $f_X(x) = \int_0^1 6xy dy = 6x \left[\frac{y^2}{2}\right]_0^1 = 6x \cdot \frac{1}{2} = 3x$

Similarly, $f_Y(y) = 3y$

\textbf{b)} $f_X(x) \cdot f_Y(y) = 3x \cdot 3y = 9xy \neq 6xy = f_{X,Y}(x,y)$

Not independent.

\subsection*{Problem 4}
Event $A$: $P(5 \text{ or } 6) = \frac{2}{6} = \frac{1}{3}$

Event $B$: $P\{(3,6), (4,6), (5,6), (6,6), (6,3), (6,4), (6,5), (5,5), (2,5), (2,2)\} = \frac{10}{36}$

$P(B|A) = \frac{P(A \cap B)}{P(A)}$

$|A \cap B| = |\{(5,4), (5,5), (5,6), (6,3), (6,4), (6,5), (6,6)\}| = 7$

$\frac{7/36}{2/6} = \frac{7/36}{1/3} = \frac{7}{12}$

\subsection*{Problem 5}
Random variable $X$ with pdf $f(x) = 3(1-x)^2$, $Y = (1-X)^{1/3}$

$Y^{1/3} = 1-X$, so $X = 1-Y^{1/3}$

$\frac{dx}{dy} = -\frac{1}{3}Y^{-2/3}$

$f_Y(y) = f_X(1-y^{1/3}) \left|\frac{dx}{dy}\right| = 3(1-(1-y^{1/3}))^2 \cdot \frac{1}{3}y^{-2/3} = 3(y^{1/3})^2 \cdot \frac{1}{3}y^{-2/3} = 1$

$f_Y(y) = \begin{cases} 1 & 0 \leq y \leq 1 \\ 0 & \text{otherwise} \end{cases}$

\subsection*{Problem 6}
$\text{Cov}\left(\sum_{i=1}^n a_i X_i, \sum_{j=1}^n a_j X_j\right) = \sum_{i=1}^n \sum_{j=1}^n a_i a_j \text{Cov}(X_i, X_j) = a^T S a$

$Y = \sum_{i=1}^n a_i X_i$, $Z = \sum_{j=1}^n a_j X_j$

$E(Y) = E\left(\sum_{i=1}^n a_i X_i\right) = \sum_{i=1}^n a_i E(X_i)$

$E(Z) = \sum_{j=1}^n a_j E(X_j)$

$\text{Cov}(Y,Z) = E(YZ) - E(Y)E(Z)$

$= \sum_{i=1}^n \sum_{j=1}^n a_i a_j E(X_i X_j) - \sum_{i=1}^n a_i E(X_i) \sum_{j=1}^n a_j E(X_j)$

$= \sum_{i=1}^n \sum_{j=1}^n a_i a_j [E(X_i X_j) - E(X_i)E(X_j)]$

$= \sum_{i=1}^n \sum_{j=1}^n a_i a_j \text{Cov}(X_i, X_j)$

$a^T S a = \sum_{i=1}^n \sum_{j=1}^n a_i S_{ij} a_j = \sum_{i=1}^n \sum_{j=1}^n a_i a_j \text{Cov}(X_i, X_j)$

\subsection*{Problem 7}
$f(x) = \log(1 + e^x)$, $\sigma(x) = \frac{e^x}{1 + e^x}$

\textbf{(1)} $\frac{d f(x)}{dx} = \frac{1}{1+e^x} \cdot \frac{d}{dx}(1+e^x) = \frac{e^x}{1+e^x}$

\textbf{(2)} $\frac{d\sigma(x)}{dx} = \frac{d}{dx}\left(\frac{e^x}{1+e^x}\right) = \frac{e^x(1+e^x) - e^x \cdot e^x}{(1+e^x)^2} = \frac{e^x}{(1+e^x)^2} = \sigma(x) \cdot \frac{1}{1+e^x} = \sigma(x)(1-\sigma(x))$

\textbf{(3)} $\log(\sigma(x)) = \log\left(\frac{e^x}{1+e^x}\right) = \log(e^x) - \log(1+e^x) = x - f(x)$

\textbf{(4)} $1-\sigma(x) = 1 - \frac{e^x}{1+e^x} = \frac{1+e^x-e^x}{1+e^x} = \frac{1}{1+e^x}$

$\sigma(-x) = \frac{e^{-x}}{1+e^{-x}} = \frac{1}{e^x+1} = 1-\sigma(x)$

\textbf{(5)} $\sigma^{-1}(x) = \log\left(\frac{x}{1-x}\right)$

Let $y = \sigma(x) = \frac{e^x}{1+e^x}$

$y(1+e^x) = e^x$
$y + ye^x = e^x$
$y = e^x(1-y)$
$e^x = \frac{y}{1-y}$
$x = \log\left(\frac{y}{1-y}\right)$

\textbf{(6)} $\log(\sigma(x)) = -f(-x)$

$\log\left(\frac{1}{1+e^{-x}}\right) = \log(e^x) - \log(1+e^x) = x - \log(1+e^x) = x - f(x) = -f(-x)$

\textbf{(7)} $f(x) = \int_{-\infty}^x \sigma(y) dy$

Let $u = 1+e^y$, $du = e^y dy$

$\int \frac{e^y}{1+e^y} dy = \int \frac{1}{u} du = \ln(u) = \ln(1+e^y)$

$\int_{-\infty}^x \sigma(y) dy = \ln(1+e^x) - \ln(1+e^{-\infty}) = \ln(1+e^x) - \ln(1) = \ln(1+e^x) = f(x)$

\textbf{(8)} $f(x) - f(-x) = x$

$f(x) - f(-x) = \log(1+e^x) - \log(1+e^{-x}) = \log(1+e^x) - \log\left(\frac{e^x+1}{e^x}\right) = \log(1+e^x) - \log(e^x+1) + x = x$

\end{document}
```